AP/Util/Data/Trie/Trie.lean
@@ -29,45 +29,573 @@ def depth (t : Trie α β) : ℕ :=
 theorem depth_empty : (∅ : Trie α β).depth = 0 := by
   simp [depth, empty_def, empty]
 
-theorem option_map_ofRaw_get?_eq_of_equiv {a b : Raw α β} {k}
-(h₁ : a.Equiv b) : Option.map ofRaw (a.get? k) = Option.map ofRaw (b.get? k) := by
+theorem option_map_ofRaw_get1?_eq_of_equiv {a b : Raw α β} {k}
+(h₁ : a.Equiv b) : Option.map ofRaw (a.get1? k) = Option.map ofRaw (b.get1? k) := by
   ext c
   rcases c with ⟨c⟩
   simp
   constructor <;> rintro ⟨c, h₂, rfl⟩
-  · replace h₂ := h₁.get? h₂
+  · replace h₂ := h₁.get1? h₂
     choose d h₂ h₃ using h₂
     use d, h₂
     simpa
-  · replace h₂ := h₁.get?' h₂
+  · replace h₂ := h₁.get1?' h₂
     choose d h₂ h₃ using h₂
     use d, h₂
     simpa
 
-def get? (t : Trie α β) (k : α) : Option (Trie α β) :=
-  t.inner.lift (λ t => t.get? k |>.map ofRaw) # λ _ _ => option_map_ofRaw_get?_eq_of_equiv
+def get1? (t : Trie α β) (k : α) : Option (Trie α β) :=
+  t.inner.lift (λ t => t.get1? k |>.map ofRaw) # λ _ _ => option_map_ofRaw_get1?_eq_of_equiv
 
-theorem depth_lt {k} (h : t.get? k = some t') : t'.depth < t.depth := by
+theorem depth_lt {k} (h : t.get1? k = some t') : t'.depth < t.depth := by
   rcases t, t' with ⟨⟨t⟩, ⟨t'⟩⟩
   revert h
   induction t, t' using Quotient.inductionOn₂
   nm t t'
-  simp [get?, depth]
+  simp [get1?, depth]
   intro a h₁ (h₂ : a.Equiv t')
   rw [←h₂.depth_eq]
   exact Raw.depth_lt h₁
 
-def eqComp (t₁ t₂ : Trie α β) : Bool :=
+def eqComp [hb : DecidableEq β] (t₁ t₂ : Trie α β) : Bool :=
   t₁.inner.liftOn₂ t₂.1 Raw.equivComp Raw.equivComp_eq_of_equiv2_expl
 
-theorem eq_iff_eqComp : t₁ = t₂ ↔ t₁.eqComp t₂ := by
+theorem eq_iff_eqComp [hb : DecidableEq β] : t₁ = t₂ ↔ t₁.eqComp t₂ := by
   rcases t₁, t₂ with ⟨⟨t⟩, ⟨t'⟩⟩
   induction t, t' using Quotient.inductionOn₂
   simp [eqComp]; rfl
 
-instance : DecidableEq (Trie α β) :=
+instance [hb : DecidableEq β] : DecidableEq (Trie α β) :=
   λ _ _ => decidable_of_bool _ eq_iff_eqComp.symm
 
 @[simp]
-theorem eqComp_iff_decide_eq : t₁.eqComp t₂ ↔ decide (t₁ = t₂) := by
+theorem eqComp_iff_decide_eq [hb : DecidableEq β] : t₁.eqComp t₂ ↔ decide (t₁ = t₂) := by
   simp [eq_iff_eqComp]
+
+def val (t : Trie α β) : Option β :=
+  t.1.lift Raw.val # λ _ _ => Raw.Equiv.val_eq
+
+#check 0 #exit
+
+def insert1 (t : Trie α β) (i : List α) (x : β) : Trie α β :=
+
+#check 0 #exit
+
+protected def insert (t : Trie α β) (is : List α) (x : β) : Trie α β :=
+
+#check 0 #exit
+
+def insertP (x : α × β) (mp : Map α β) : Map α β :=
+  ⟨insert x.toSigma mp.inner⟩
+
+instance : Insert (α × β) (Map α β) := ⟨insertP⟩
+
+theorem insert_def {x : α × β} {mp : Map α β} :
+insert x mp = ⟨insert x.toSigma mp.inner⟩ := rfl
+
+protected def insert (mp : Map α β) (i : α) (x : β) : Map α β :=
+  ⟨mp.inner.insert i x⟩
+
+def ofList (xs : List (α × β)) : Map α β :=
+  ⟨.ofList # xs.map Prod.toSigma⟩
+
+def get? (i : α) (mp : Map α β) : Option β :=
+  mp.inner.get1? i
+
+def get! (i : α) [h : Inhabited β] (mp : Map α β) : β :=
+  mp.inner.get! i
+
+def map (mp : Map α β) (f : α → β → γ) : Map α γ :=
+  ⟨mp.inner.map f⟩
+
+def mem (mp : Map α β) (i : α) : Prop :=
+  i ∈ mp.inner
+
+instance : Membership α (Map α β) := ⟨mem⟩
+
+theorem mem_def {i} : i ∈ mp ↔ i ∈ mp.inner := by rfl
+
+instance {i} : Decidable (mp.mem i) := by
+  unfold mem; infer_instance
+
+instance {i} : Decidable (i ∈ mp) := by
+  change Decidable # mp.mem i; infer_instance
+
+theorem mem_iff_get?_eq_some {i : α} : i ∈ mp ↔ ∃ x, mp.get1? i = some x :=
+  Std.ExtDHashMap.mem_iff_get?_eq_some
+
+theorem get?_eq_some_of_mem {i : α} (h : i ∈ mp) : ∃ x, mp.get1? i = some x :=
+  Std.ExtDHashMap.get1?_eq_some_of_mem h
+
+theorem get?_eq_none_of_not_mem {i : α} (h : i ∉ mp) : mp.get1? i = none :=
+  Std.ExtDHashMap.get1?_eq_none_of_not_mem h
+
+@[simp]
+theorem get?_eq_none_iff {i} : mp.get1? i = none ↔ i ∉ mp :=
+  Std.ExtDHashMap.get1?_eq_none_iff
+
+theorem get?_map {f : α → β → γ} {i : α} :
+(mp.map f).get1? i = (mp.get1? i).map (f i) :=
+  Std.ExtDHashMap.get1?_map
+
+theorem get!_map_eq_of_pos {f : α → β → γ} {i : α}
+[ha : Inhabited β] [hb : Inhabited γ]
+(h : i ∈ mp) : (mp.map f).get! i = f i (mp.get! i) := by
+  rcases mp with ⟨⟨mp⟩⟩
+  obtain ⟨x, hx⟩ := get?_eq_some_of_mem h
+  induction mp using Quotient.inductionOn
+  simp [get?] at hx
+  simp [get!, Std.ExtDHashMap.get!_eq_get?, map, hx]
+
+def toList [LinearOrder α] (mp : Map α β) : List (α × β) :=
+  mp.inner.lift (λ m => m.toSortedList.map Sigma.toProd) #
+    by simp
+
+@[simp]
+theorem ofList_nil : ofList (α := α) (β := β) [] = ∅ := rfl
+
+@[simp]
+theorem ofList_snoc {xs} {x : α × β} :
+ofList (xs ++ [x]) = (ofList xs).insertP x := by
+  unfold insertP ofList; simp
+
+@[simp]
+theorem toList_empty [LinearOrder α] : (∅ : Map α β).toList = [] := by
+  change List.map _ _ = _; simp [toSortedList]
+
+@[simp]
+theorem mem_insertP {x : α × β} {i} :
+i ∈ mp.insertP x ↔ i = x.1 ∨ i ∈ mp :=
+  Std.ExtDHashMap.mem_insert'
+
+@[simp]
+theorem mem_insert' {i x j} : j ∈ mp.insert i x ↔ j = i ∨ j ∈ mp := by
+  simp [mem_def, Map.insert]; tauto
+
+@[simp]
+theorem mem_insert {x i} : i ∈ Insert.insert x mp ↔ i = x.1 ∨ i ∈ mp :=
+  mem_insert'
+
+@[simp]
+theorem mem_ofList {xs : List (α × β)} {i} :
+i ∈ ofList xs ↔ ∃ x, ⟨i, x⟩ ∈ xs := by
+  induction xs using List.ind_pair_sigma; simp [ofList]
+  exact Std.ExtDHashMap.mem_ofList'
+
+@[simp]
+theorem mem_map {f : α → β → γ} {i} :
+i ∈ mp.map f ↔ i ∈ mp := by
+  simp [mem_def, map]
+
+theorem eq_empty_iff : mp = ∅ ↔ ∀ i, i ∉ mp := by
+  rcases mp with ⟨mp⟩; simp [empty_def]
+  exact Std.ExtDHashMap.eq_empty_iff
+
+@[simp]
+theorem not_mem_empty' {i} : ¬(∅ : Map α β).mem i :=
+  Std.ExtDHashMap.not_mem_empty
+
+@[simp]
+theorem not_mem_empty {i} : i ∉ (∅ : Map α β) :=
+  not_mem_empty'
+
+theorem ext_iff' {m₁ m₂ : Map α β} :
+m₁ = m₂ ↔ m₁.inner.1.out ~m m₂.inner.1.out := by
+  rcases m₁ with ⟨m₁⟩; rcases m₂ with ⟨m₂⟩; simp
+  exact Std.ExtDHashMap.ext_iff'
+
+theorem ext' {m₁ m₂ : Map α β}
+(h : m₁.inner.1.out ~m m₂.inner.1.out) : m₁ = m₂ := by
+  rwa [ext_iff']
+
+theorem ext_iff {m₁ m₂ : Map α β} : m₁ = m₂ ↔ ∀ i, m₁.get1? i = m₂.get1? i := by
+  rcases m₁ with ⟨m₁⟩; rcases m₂ with ⟨m₂⟩; simp
+  exact Std.ExtDHashMap.ext_iff
+
+@[ext]
+theorem ext {m₁ m₂ : Map α β} (h : ∀ i, m₁.get1? i = m₂.get1? i) : m₁ = m₂ := by
+  rwa [ext_iff]
+
+theorem get?_eq_ite_of_unit {m : Map α Unit} {i} :
+m.get1? i = if i ∈ m then some () else none :=
+  Std.ExtDHashMap.get1?_eq_ite_of_unit
+
+@[simp]
+theorem get?_empty {i} : (∅ : Map α β).get1? i = none :=
+  Std.ExtDHashMap.get1?_empty
+
+theorem ofList_eq_ofList_iff {xs ys : List (α × β)}
+(hx : (xs.map (·.1)).Nodup) (hy : (ys.map (·.1)).Nodup) :
+ofList xs = ofList ys ↔ xs.Perm ys := by
+  induction xs using List.ind_pair_sigma
+  induction ys using List.ind_pair_sigma
+  simp [ofList]
+  rw [List.map_map] at hx hy
+  rw [Std.ExtDHashMap.ofList_eq_ofList_iff hx hy]
+  rw [List.map_perm_map_iff # by simp]
+
+def range [ha : Fintype α] (f : α → β) : Map α β :=
+  ⟨Std.ExtDHashMap.range f⟩
+  
+@[simp]
+theorem mem_range [ha : Fintype α] {f : α → β} {i : α} : i ∈ range f :=
+  Std.ExtDHashMap.mem_range
+
+@[simp]
+theorem nonempty_insert {x} : Insert.insert x mp ≠ ∅ := by
+  simp [ext_iff', ←equiv_def]
+  rcases mp with ⟨mp⟩
+  rw [insert_def]
+  simp
+  have h₁ := @Std.ExtDHashMap.nonempty_insert α (λ _ => β) _ _
+    mp x.toSigma
+  simp at h₁
+  rwa [Std.ExtDHashMap.inner_eq_iff_eq]
+
+@[simp]
+theorem nodup_toList [LinearOrder α] : mp.toList.Nodup := by
+  rcases mp with ⟨⟨mp⟩⟩; unfold toList Std.ExtDHashMap.lift
+  rw [Quotient.lift_eq]
+  rw [List.nodup_map_iff # by simp]
+  simp
+
+@[simp]
+theorem sorted_toList [LinearOrder α] : mp.toList.Sorted (·.1 ≤ ·.1) := by
+  rcases mp with ⟨⟨mp⟩⟩; unfold toList Std.ExtDHashMap.lift
+  apply mp.ind; simp
+
+@[simp]
+theorem mem_toList [LinearOrder α] {x} : x ∈ mp.toList ↔ mp.get1? x.1 = x.2 := by
+  rcases mp with ⟨⟨mp⟩⟩; unfold toList
+  apply mp.ind
+  clear mp; intro mp
+  unfold toSortedList get? Std.ExtDHashMap.get1?
+  rcases x with ⟨x, y⟩
+  unfold Std.ExtDHashMap.lift
+  simp
+
+@[simp]
+theorem toList_eq_toList [LinearOrder α] {m₁ m₂ : Map α β} :
+m₁.toList = m₂.toList ↔ m₁ = m₂ := by
+  rcases m₁ with ⟨⟨m₁⟩⟩; rcases m₂ with ⟨⟨m₂⟩⟩
+  simp [Std.ExtDHashMap.lift, toList, Quotient.lift_eq, ←equiv_def]
+
+@[simp]
+theorem toList_eq_nil_iff [LinearOrder α] : mp.toList = [] ↔ mp = ∅ := by
+  rcases mp with ⟨⟨mp⟩⟩; unfold toList
+  apply mp.ind; clear mp; intro mp
+  simp [empty_def]
+  unfold Std.ExtDHashMap.lift
+  simp
+  change _ ↔ _ = Std.ExtDHashMap.mk' _
+  simp
+  change _ ↔ _ ~m _
+  simp
+
+@[simp]
+def toDMap (mp : Map α β) : DMap α (λ _ => β) :=
+  ⟨mp.inner⟩
+
+end Map namespace DMap
+
+@[simp]
+def toMap (mp : DMap α (λ _ => β)) : Map α β :=
+  ⟨mp.inner⟩
+
+end DMap namespace Map
+
+instance [hh : DecidableEq β] : DecidableEq (Map α β) :=
+  λ m₁ m₂ => match h : decide # m₁.inner = m₂.inner with
+  | true => isTrue # by
+    rcases m₁ with ⟨m₁⟩; rcases m₂ with ⟨m₂⟩
+    simp at h; simpa
+  | false => isFalse # by
+    rcases m₁ with ⟨m₁⟩; rcases m₂ with ⟨m₂⟩
+    simp at h; simpa
+
+def values [LinearOrder α] (mp : Map α β) : List β :=
+  mp.toList.map (·.2)
+
+def all (mp : Map α β) (p : α → β → Bool) : Bool :=
+  mp.1.all p
+
+@[simp]
+theorem all_def [LinearOrder α] {p} : mp.all p = decide (∀ x ∈ mp.toList, p x.1 x.2) := by
+  simp [all]; rfl
+
+def modify (mp : Map α β) (i : α) (f : β → β) : Map α β :=
+  ⟨mp.1.modify i f⟩
+
+def modifyMany (mp : Map α β) (xs : List (α × (β → β))) : Map α β :=
+  ⟨mp.1.modifyMany # xs.map (·.toSigma)⟩
+
+@[simp]
+theorem modifyMany_nil : mp.modifyMany [] = mp := by
+  simp [modifyMany]
+
+@[simp]
+theorem modifyMany_cons {i x xs} :
+mp.modifyMany ((i, x) :: xs) = (mp.modify i x).modifyMany xs := by
+  simp [modifyMany, modify]
+
+def insertMany (mp : Map α β) (xs : List (α × β)) : Map α β :=
+  ⟨mp.1.insertMany # xs.map (·.toSigma)⟩
+
+@[simp]
+theorem insertMany_nil : mp.insertMany [] = mp := by
+  simp [insertMany]
+
+@[simp]
+theorem insertMany_cons {i x xs} :
+mp.insertMany ((i, x) :: xs) = (mp.insert i x).insertMany xs := by
+  simp [insertMany, Std.ExtDHashMap.insertMany_cons, Std.ExtDHashMap.insert, Map.insert]
+
+theorem get?_eq_ite [hb : Inhabited β] {i} :
+mp.get1? i = if i ∈ mp then some # mp.get! i else none :=
+  mp.1.get1?_eq_ite
+
+@[simp]
+theorem mem_modify {i j x} : i ∈ mp.modify j x ↔ i ∈ mp :=
+  Std.ExtDHashMap.mem_modify
+
+theorem get!_eq_get?_get! [Inhabited β] {i} : mp.get! i = (mp.get1? i).get! :=
+  Std.ExtDHashMap.get!_eq_get!_get?
+
+@[simp]
+theorem get?_modify {i} {f : β → β} {j} :
+(mp.modify i f).get1? j = if j = i then
+(mp.get1? j).map f else mp.get1? j := by
+  split_ifs with h₁; subst h₁; simp [modify, get?]
+  simp [modify, get?, Std.ExtDHashMap.get1?_modify, ne_symm' h₁]
+
+@[simp]
+theorem mem_values [LinearOrder α] {x} : x ∈ mp.values ↔ ∃ i, mp.get1? i = some x := by
+  simp [values]
+
+instance [ha : Fintype α] [hb : Fintype β] : Fintype (Map α β) :=
+  haveI h : Fintype # Std.ExtDHashMap α (λ _ => β) := inferInstance
+  ⟨h.1.map ⟨.mk, λ _ _ => by simp⟩, by simp⟩
+
+instance [ha : Finite α] [hb : Finite β] : Finite (Map α β) := by
+  apply Fintype.finite
+  replace ha := @Fintype.ofFinite _ ha
+  replace hb := @Fintype.ofFinite _ hb
+  infer_instance
+
+@[simp]
+theorem range_eq_range_iff [ha : Fintype α] {f g : α → β} :
+range f = range g ↔ ∀ x, f x = g x := by simp [range]
+
+theorem mem_of_get?_eq_some {i x} (h : mp.get1? i = some x) : i ∈ mp := by
+  simp [mem_iff_get?_eq_some, h]
+
+theorem get!_eq_get!_get? {i} [hb : Inhabited β] :
+mp.get! i = (mp.get1? i).get! := Std.ExtDHashMap.get!_eq_get!_get?
+
+@[simp]
+theorem get?_eq_some_get!_iff {i} [hb : Inhabited β] :
+mp.get1? i = some (mp.get! i) ↔ i ∈ mp := by
+  simp [get?_eq_ite]
+
+@[simp]
+theorem get?_eq_some_get?_get! {i} [hb : Inhabited β] :
+mp.get1? i = some (mp.get1? i).get! ↔ i ∈ mp := by
+  simp [←get!_eq_get!_get?]
+
+def fold {γ : Type*} (mp : Map α β) (f : γ → α → β → γ) (z : γ)
+(h_assoc : ∀ {acc i x j y}, f (f acc i x) j y = f (f acc j y) i x) : γ :=
+  mp.inner.fold f z h_assoc
+
+theorem fold_eq_foldl_toList [ha : LinearOrder α] {γ : Type*}
+{z : γ} {f : γ → α → β → γ} {h_assoc} : mp.fold f z h_assoc =
+mp.toList.foldl (λ acc (x : α × β) => f acc x.1 x.2) z := by
+  convert Std.ExtDHashMap.fold_eq_foldl_toList; rotate_left; infer_instance
+  simp [toList, Std.ExtDHashMap.toList, Std.ExtDHashMap.lift]
+  rcases mp with ⟨⟨mp⟩⟩
+  simp
+  apply mp.ind
+  simp [List.foldl_map]
+
+theorem eq_iff_inner_eq {m₁ m₂ : Map α β} : m₁ = m₂ ↔ m₁.inner = m₂.inner := by
+  rcases m₁, m₂ with ⟨⟨m₁⟩, ⟨m₂⟩⟩; simp
+
+theorem eq_iff_toList_eq [ha : LinearOrder α] {m₁ m₂ : Map α β} :
+m₁ = m₂ ↔ m₁.toList = m₂.toList := by
+  rcases m₁, m₂ with ⟨⟨m₁⟩, ⟨m₂⟩⟩; simp
+
+@[simp]
+theorem ofList_toList [ha : LinearOrder α] : ofList mp.toList = mp := by
+  rw [eq_iff_inner_eq]
+  rw [←Std.ExtDHashMap.ofList_toList (mp := mp.inner)]
+  unfold ofList
+  dsimp
+  rcases mp with ⟨⟨mp⟩⟩
+  simp [toList, Std.ExtDHashMap.lift]
+  apply mp.ind
+  intro m
+  simp
+  rw [Std.ExtDHashMap.eq_iff_inner_eq]
+  simp
+  apply Quotient.eq_iff_equiv.mpr
+  apply Std.DHashMap.equiv_iff_toList_perm.mpr
+  trans m.toSortedList
+  rotate_left; simp
+  apply Std.DHashMap.toList_ofList_perm
+  simp
+
+theorem toList_ofList_perm [ha : LinearOrder α] {xs : List (α × β)}
+(h : xs.map (·.1) |>.Nodup) : (ofList xs).toList.Perm xs := by
+  generalize hy : xs.map Prod.toSigma = ys
+  have hx : ys.map Sigma.toProd = xs; simp [←hy]
+  subst hx; clear hy; rename' ys => xs
+  simp at h
+  trans (DMap.ofList xs).toList.map Sigma.toProd
+  rotate_left
+  · rw [List.map_perm_map_iff # by simp]
+    exact DMap.toList_ofList_perm h
+  simp [ofList]; rfl
+
+def keys [ha : LinearOrder α] (mp : Map α β) : List α :=
+  mp.inner.keys
+
+@[simp]
+theorem sorted_keys [ha : LinearOrder α] : mp.keys.Sorted (· ≤ ·) :=
+  Std.ExtDHashMap.sorted_keys
+
+theorem keys_eq_map_fst_toList [ha : LinearOrder α] : mp.keys = mp.toList.map (·.1) := by
+  rcases mp with ⟨mp⟩; simp [keys, toList, Std.ExtDHashMap.lift]; symm
+  refine' Quotient.apply_lift (f := List.map # λ (x : α × β) => x.1) _ |>.trans _
+  intro m₁ m₂ h₁; simp; exact Std.DHashMap.toSortedKeys_eq_of_equiv h₁; simp; rfl
+
+def minKey? [ha : LinearOrder α] (mp : Map α β) : Option α :=
+  mp.inner.minKey?
+
+def maxKey? [ha : LinearOrder α] (mp : Map α β) : Option α :=
+  mp.inner.maxKey?
+
+def minKey! [Inhabited α] [ha : LinearOrder α] (mp : Map α β) : α :=
+  mp.minKey?.get!
+
+def maxKey! [Inhabited α] [ha : LinearOrder α] (mp : Map α β) : α :=
+  mp.maxKey?.get!
+
+theorem minKey?_eq_head?_keys [ha : LinearOrder α] : mp.minKey? = mp.keys.head? :=
+  Std.ExtDHashMap.minKey?_eq_head?_keys
+
+theorem maxKey?_eq_getLast?_keys [ha : LinearOrder α] : mp.maxKey? = mp.keys.getLast? :=
+  Std.ExtDHashMap.maxKey?_eq_getLast?_keys
+
+@[simp]
+theorem minKey?_eq_none_iff [ha : LinearOrder α] : mp.minKey? = none ↔ mp = ∅ := by
+  rw [eq_iff_inner_eq]; exact Std.ExtDHashMap.minKey?_eq_none_iff
+
+@[simp]
+theorem maxKey?_eq_none_iff [ha : LinearOrder α] : mp.maxKey? = none ↔ mp = ∅ := by
+  rw [eq_iff_inner_eq]; exact Std.ExtDHashMap.maxKey?_eq_none_iff
+
+theorem not_mem_of_lt_minKey? [ha : LinearOrder α] {m x}
+(h₁ : mp.minKey? = some m) (h₂ : x < m) : x ∉ mp :=
+  Std.ExtDHashMap.not_mem_of_lt_minKey? h₁ h₂
+
+theorem not_mem_of_maxKey?_lt [ha : LinearOrder α] {m x}
+(h₁ : mp.maxKey? = some m) (h₂ : m < x) : x ∉ mp :=
+  Std.ExtDHashMap.not_mem_of_maxKey?_lt h₁ h₂
+
+theorem not_mem_of_lt_minKey! [ha₁ : Inhabited α] [ha₂ : LinearOrder α] {x}
+(h : x < mp.minKey!) : x ∉ mp := Std.ExtDHashMap.not_mem_of_lt_minKey! h
+
+theorem not_mem_of_maxKey!_lt [ha₁ : Inhabited α] [ha₂ : LinearOrder α] {x}
+(h : mp.maxKey! < x) : x ∉ mp := Std.ExtDHashMap.not_mem_of_maxKey!_lt h
+
+theorem minKey?_le_of_mem [ha : LinearOrder α] {m x}
+(h₁ : mp.minKey? = some m) (h₂ : x ∈ mp) : m ≤ x := by
+  contrapose! h₂; exact not_mem_of_lt_minKey? h₁ h₂
+
+theorem le_maxKey?_of_mem [ha : LinearOrder α] {m x}
+(h₁ : mp.maxKey? = some m) (h₂ : x ∈ mp) : x ≤ m := by
+  contrapose! h₂; exact not_mem_of_maxKey?_lt h₁ h₂
+
+theorem minKey!_le_of_mem [ha₁ : Inhabited α] [ha₂ : LinearOrder α] {x}
+(h : x ∈ mp) : mp.minKey! ≤ x := by
+  contrapose! h; exact not_mem_of_lt_minKey! h
+
+theorem le_maxKey!_of_mem [ha₁ : Inhabited α] [ha₂ : LinearOrder α] {x}
+(h : x ∈ mp) : x ≤ mp.maxKey! := by
+  contrapose! h; exact not_mem_of_maxKey!_lt h
+
+theorem ind {p : Map α β → Prop} (h₁ : p ∅)
+(h₂ : ∀ (m : Map α β) i x, p m → i ∉ m → p (m.insert i x)) m : p m := by
+  rcases m with ⟨mp⟩; induction mp using Std.ExtDHashMap.ind
+  exact h₁; apply h₂ <;> assumption
+
+@[simp]
+theorem fold_empty {γ : Type*} {f : γ → (i : α) → β → γ} {z : γ} {h} :
+(∅ : Map α β).fold f z h = z := Std.ExtDHashMap.fold_empty
+
+theorem fold_insert {γ : Type*} {f : γ → α → β → γ} {z : γ} {h i x}
+(h₁ : i ∉ mp) : (mp.insert i x).fold f z h = mp.fold f (f z i x) h :=
+  Std.ExtDHashMap.fold_insert # by simpa
+
+theorem insert_comm {i x j y} (h : i ≠ j ∨ x = y) :
+(mp.insert i x).insert j y = (mp.insert j y).insert i x := by
+  simp [Map.insert]; apply Std.ExtDHashMap.insert_comm; simpa
+
+@[simp]
+theorem insert_idemp {i x} : (mp.insert i x).insert i x = mp.insert i x := by
+  simp [Map.insert]
+
+def size (mp : Map α β) : ℕ :=
+  mp.1.size
+
+def filter (mp : Map α β) (p : α → β → Bool) : Map α β :=
+  ⟨mp.1.filter p⟩
+
+def count (mp : Map α β) (p : α → β → Bool) : ℕ :=
+  mp.1.count p
+
+@[simp]
+theorem size_filter_eq_count {p} : (mp.filter p).size = mp.count p :=
+  mp.1.size_filter_eq_count
+
+theorem count_eq_size_filter {p} : mp.count p = (mp.filter p).size :=
+  size_filter_eq_count.symm
+
+@[simp]
+theorem count_le_size {p} : mp.count p ≤ mp.size :=
+  mp.1.count_le_size
+
+theorem count_eq_zero_iff {p} :
+mp.count p = 0 ↔ ∀ i x, mp.get1? i = some x → ¬p i x :=
+  mp.1.count_eq_zero_iff
+
+@[simp]
+theorem count_empty {p} : (∅ : Map α β).count p = 0 :=
+  Std.ExtDHashMap.count_empty
+
+theorem count_insert {p i x} (h : i ∉ mp) :
+(mp.insert i x).count p = mp.count p + if p i x then 1 else 0 :=
+  mp.1.count_insert h
+
+def push (mp : Map α ℕ) (i : α) : Map α ℕ :=
+  mp.insert i # (mp.get1? i).getD 0 + 1
+
+theorem get?_insert {i j x} :
+(mp.insert j x).get1? i = if j = i then some x else mp.get1? i := by
+  convert mp.1.get1?_insert; simp; rfl
+
+theorem push_push_comm {i j} {mp : Map α ℕ} :
+(mp.push i).push j = (mp.push j).push i := by
+  ext; simp [push, get?_insert]; aesop
+
+@[simp]
+theorem mem_push {mp : Map α ℕ} {x y : α} : y ∈ mp.push x ↔ y = x ∨ y ∈ mp := by
+  simp [push]
+
+@[simp]
+theorem length_toList [ha : LinearOrder α] : mp.toList.length = mp.size := by
+  rcases mp with ⟨m⟩
+  simp [toList, size, Std.ExtDHashMap.lift, Std.ExtDHashMap.size]
+  induction m; simp
+
+theorem mem_iff_mem_keys [ha : LinearOrder α] {k} : k ∈ mp ↔ k ∈ mp.keys := by
+  simp [keys_eq_map_fst_toList, mem_iff_get?_eq_some]
